---
title: "Taylor Series - Assignment 14"
author: "Sharon Morris"
date: "4/27/2017"
output:
  pdf_document: 
    latex_engine: lualatex
  html_document: default
---

For each function, only consider its valid ranges as indicated in the notes when you are computing the Taylor Series expansion.

1) $f(x)= \frac{1}{1-x}$

$f'(x)=(-1)(-1)(1-x)^-2=1$
$f''(x)=(-1^2)(-1)(-2)(1-x)^-3=2$
$f'''(x)=(-1^3)(-1)(-2)(-3)(1-x)^-4=6$
$f^n(x)=(n!)(1-x)^-n$

Talor Series expansion $\frac{1}{(1-x)}$
$f(x)= \sum_{n \to 0} ^{\infty}\frac{f^n(a)}{n!}(x-a)^n$
$f(x)=1+x+x^2+x^3+x^4+...$


2.) $f(x)=e^x$

$f(x)= \sum_{n \to 0} ^{\infty}\frac{f^n(a)}{n!}(x-a)^n$
$f(x)=1+x+\frac{x^2}{2!}+\frac {x^3}{3!}+\frac {x^4}{4!}+...$



3) $f(x)=ln(1+x)$

$f'(x)=\frac{1}{(1+x)}=1$
$f''(x)=(-1)(1+x)^-2=-1$
$f'''(x)=(-1)(-2)(1+x)^-3=2$

Talor Series
$f(x)= \sum_{n \to 0} ^{\infty}\frac{f^n(a)}{n!}(x-a)^n$
$f(x)= \sum_{n \to 0} ^{\infty}\frac{(-1)^n}{n+1}x(n+1)$
$f(x)=x-\frac{x^2}{2}+\frac {x^3}{3}+\frac {x^4}{4}+...$


References
http://mathworld.wolfram.com/TaylorSeries.html


